consolidation

coq/HFT_Defns.v
@@ -1,32 +1,44 @@
-Require Import Packet.
 Require Import Coq.Lists.List.
 Require Import Coq.Arith.MinMax.
 Require Import Coq.Classes.Equivalence.
-Require Import Action.
+Require Import Coq.Classes.EquivDec.
+Require Import Impl.
 Require Import CpdtTactics.
 Require Import Omega.
+Require Import Coq.Bool.Bool.
+Require Classifier.
 
-Module Make (P : Packet).
+Inductive A : Type :=
+| NoAction : A
+| Allow : A
+| Deny : A
+| GMB : nat -> A.
 
-  Include P.
+Record pkt : Set := mkPkt {
+  pktSrcHost : nat;
+  pktDstHost : nat;
+  pktSrcPort : nat;
+  pktDstPort : nat
+}.
 
-  Inductive A : Type :=
-    | ActionUnit : A
-    | Allow : A
-    | Deny : A
-    | GMB : nat -> A.
+Inductive patElt : Set := 
+  | PatSrcHost : nat -> patElt
+  | PatDstHost : nat -> patElt
+  | PatSrcPort : nat -> patElt
+  | PatDstPort : nat -> patElt.
 
-  Lemma A_eq_dec : forall (a1 a2 : A), { a1 = a2 } + { a1 <> a2 }.
-  Proof. repeat decide equality. Qed.
+Definition pat := list patElt.
 
-  Inductive A_equiv : A -> A -> Prop :=
-  | ActionUnit_equiv : A_equiv ActionUnit ActionUnit
-  | Allow_equiv : A_equiv Allow Allow
-  | Deny_equiv : A_equiv Deny Deny
-  | GMB_equiv : forall n, A_equiv (GMB n) (GMB n).
+Inductive A_equiv : A -> A -> Prop :=
+| None_equiv : A_equiv NoAction NoAction
+| Allow_equiv : A_equiv Allow Allow
+| Deny_equiv : A_equiv Deny Deny
+| GMB_equiv : forall n, A_equiv (GMB n) (GMB n).
+
+Section Equiv.
 
   Hint Constructors A_equiv.
-
+  
   Lemma A_equiv_is_equivalence : Equivalence A_equiv.
   Proof with auto.
     crush.
@@ -40,25 +52,154 @@ Module Make (P : Packet).
     intros. destruct y; inversion H; inversion H0; subst...
   Qed.
 
-  Open Local Scope equiv_scope.
+End Equiv.
 
-  Definition well_behaved (f : A -> A -> A) : Prop :=
-    (forall (a : A), f a ActionUnit === a) /\
-    (forall (a : A), f ActionUnit a === a) /\
-    (forall a a' b b', f a b === f a' b').
+Open Local Scope equiv_scope.
 
-  Module A_as_Action <: ACTION.
-    Definition A := A.
-    Definition ActionUnit := ActionUnit.
-    Definition equiv := A_equiv.
-    Instance A_Equivalence : Equivalence equiv.
-    exact A_equiv_is_equivalence.
-    Qed.
-  Definition well_behaved (f : A -> A -> A) : Prop :=
+Definition well_behaved (f : A -> A -> A) : Prop :=
+  (forall (a : A), f a NoAction === a) /\
+  (forall (a : A), f NoAction a === a) /\
+  (forall a a' b b', a === a' -> b === b' -> f a b === f a' b').
+
+Lemma pkt_eq_dec : forall (p p' : pkt), { p = p' } + { p <> p' }.
+Proof. repeat decide equality. Qed.
+
+Lemma pat_eq_dec : forall (p p' : pat), { p = p' } + { p <> p' }.
+Proof. repeat decide equality. Qed.
+
+Inductive patElt_equiv : patElt -> patElt -> Prop :=
+ | SrcHostEquiv : forall n, patElt_equiv (PatSrcHost n) (PatSrcHost n)
+ | DstHostEquiv : forall n, patElt_equiv (PatDstHost n) (PatDstHost n)
+ | SrcPortEquiv : forall n, patElt_equiv (PatSrcPort n) (PatSrcPort n)
+ | DstPortEquiv : forall n, patElt_equiv (PatDstPort n) (PatDstPort n).
+
+Hint Constructors patElt_equiv.
+
+Open Local Scope equiv_scope.
+Instance PatElt_Equivalence : Equivalence patElt_equiv.
+Proof with auto.
+  crush.
+  unfold Reflexive. intros. destruct x; crush.
+  unfold Symmetric. intros. destruct x; destruct y; 
+    try solve [ inversion H | 
+ assert ({ n = n0 } + { ~ n = n0 }) by (apply eq_nat_dec); destruct H0; 
+   subst; auto; inversion H; subst; contradiction n1; auto ].
+  unfold Transitive.
+  intros. destruct y; inversion H; inversion H0; subst...
+Qed.
+
+Definition beq_patElt p1 p2 := match (p1, p2) with
+ | (PatSrcHost n, PatSrcHost n') => beq_nat n n'
+ | (PatDstHost n, PatDstHost n') => beq_nat n n'
+ | (PatSrcPort n, PatSrcPort n') => beq_nat n n'
+ | (PatDstPort n, PatDstPort n') => beq_nat n n'
+ | _ => false
+end.
+
+Fixpoint intersect (p : pat) (p' : pat) := 
+  match p' with
+    | nil => nil
+    | (elt :: rest) =>
+      if existsb (fun elt' => beq_patElt elt elt') p then
+        elt :: (intersect p rest)
+        else
+          intersect p rest
+  end.
+
+Definition is_overlapped (p1 : pat) (p2 : pat) : bool :=
+  match (intersect p1 p2) with
+    | nil => false
+    | _ => true
+  end.
+
+Definition exact_match (k : pkt)  :=
+  cons (PatSrcHost (pktSrcHost k))
+    (cons (PatDstHost (pktDstHost k))
+      (cons (PatSrcPort (pktSrcPort k))
+        (cons (PatDstPort (pktDstPort k)) nil))).
+
+Definition match_elt (k : pkt) (t : patElt) := match t with
+  | (PatSrcHost n) => beq_nat (pktSrcHost k) n
+  | (PatDstHost n) => beq_nat (pktDstHost k) n
+  | (PatSrcPort n) => beq_nat (pktSrcPort k) n
+  | (PatDstPort n) => beq_nat (pktDstPort k) n
+ end.
+
+Fixpoint is_match (k : pkt) (t : pat) := match t with
+  | nil => true
+  | (hd :: tl) => andb (match_elt k hd) (is_match k tl)
+end.
+
+Lemma is_match_inv : forall k t,
+  is_match k t = false ->
+  (exists e : patElt, In e t /\ match_elt k e = false).
+Proof with (auto with datatypes).
+  intros.
+  induction t.
+  inversion H.
+  simpl in H.
+  apply andb_false_iff in H.
+  destruct H.
+  exists a...
+  apply IHt in H.
+  destruct H as [e [H H']].
+  exists e...
+Qed.
+
+Lemma no_match_subset_r : forall k t' t,
+  is_match k t = false ->
+  is_match k (intersect t' t) = false.
+Proof with (auto with datatypes).
+  intros.
+  apply is_match_inv in H.
+  destruct H as [e [H H']].
+(*  generalize dependent e. *)
+  induction t'; intros.
+Admitted.
+
+Lemma no_match_subset_l : forall k t t',
+  is_match k t = false ->
+  is_match k (intersect t t') = false.
+Proof.
+Admitted.
+
+Lemma pkt_match_intersect : forall k t t',
+  is_match k t = true ->
+  is_match k t' = true ->
+  is_match k (intersect t t') = true.
+Proof with auto.
+  intros.
+Admitted.
+
+Lemma packet_split : forall k t t',
+  is_overlapped t t' = false ->
+  is_match k t = true ->
+  is_match k t' = false.
+Admitted.
+
+Module HFT_Impl <: IMPL.
+
+  Definition A := A.
+  Definition pkt := pkt.
+  Definition pat := pat.
+  Definition ActionUnit := NoAction.
+  Definition equiv := A_equiv.
+  Program Instance A_Equivalence : Equivalence equiv := A_equiv_is_equivalence.
+ Definition well_behaved (f : A -> A -> A) : Prop :=
     (forall (a : A), f a ActionUnit === a) /\
     (forall (a : A), f ActionUnit a === a) /\
     (forall (a a' b b' : A), a === a' -> b === b' -> f a b === f a' b').
-  End A_as_Action.
+  Definition pkt_eq_dec := pkt_eq_dec.
+  Definition pat_eq_dec := pat_eq_dec.
+  Definition intersect := intersect.
+  Definition is_overlapped := is_overlapped.
+  Definition is_match := is_match.
+  Definition exact_match := exact_match.
+  Definition no_match_subset_l := no_match_subset_l.
+  Definition no_match_subset_r := no_match_subset_r.
+  Definition pkt_match_intersect := pkt_match_intersect.
+  Definition packet_split := packet_split.
+End HFT_Impl.
 
 Definition S : Type := list (pat * A).
 
@@ -72,9 +213,9 @@ Inductive wf_tree : nat -> T -> Prop :=
     (forall (t' : T), In t' lst -> wf_tree n t') ->
     wf_tree (Datatypes.S n) (Tree s lst).
 
-Definition plus_P (a1 : A_as_Action.A) (a2 : A_as_Action.A) : A_as_Action.A := match (a1, a2) with
-  | (_, ActionUnit) => a1
-  | (ActionUnit, _) => a2
+Definition plus_P (a1 : A) (a2 : A)  := match (a1, a2) with
+  | (_, NoAction) => a1
+  | (NoAction, _) => a2
   | (Deny, Allow) => Allow
   | (Allow, Allow) => Allow
   | (_, Deny) => Deny
@@ -84,9 +225,17 @@ Definition plus_P (a1 : A_as_Action.A) (a2 : A_as_Action.A) : A_as_Action.A := m
   | (GMB m, Allow) => GMB m
   end.
 
-Definition plus_S (a1 : A_as_Action.A) (a2 : A_as_Action.A) : A_as_Action.A := match (a1, a2) with
-  | (_, ActionUnit) => a1
-  | (ActionUnit, _) => a2
+Lemma well_behaved_plus_P : HFT_Impl.well_behaved plus_P.
+Proof.
+  split. intros a; destruct a; apply reflexivity.
+  split. intros a; destruct a; apply reflexivity.
+  intros. destruct a ; destruct b; destruct a'; destruct b';
+  inversion H0; inversion H; reflexivity.
+Qed.
+
+Definition plus_S (a1 a2 : A) := match (a1, a2) with 
+  | (_, NoAction) => a1
+  | (NoAction, _) => a2
   | (Deny, _) => Deny
   | (_, Deny) => Deny
   | (GMB m, GMB n) => GMB (max m n)
@@ -95,7 +244,7 @@ Definition plus_S (a1 : A_as_Action.A) (a2 : A_as_Action.A) : A_as_Action.A := m
   | (Allow, Allow) => Allow
   end.
 
-Lemma well_behaved_plus_P : A_as_Action.well_behaved plus_P.
+Lemma well_behaved_plus_S : HFT_Impl.well_behaved plus_S.
 Proof.
   split. intros a; destruct a; apply reflexivity.
   split. intros a; destruct a; apply reflexivity.
@@ -103,20 +252,10 @@ Proof.
   inversion H0; inversion H; reflexivity.
 Qed.
 
-Lemma well_behaved_plus_S : A_as_Action.well_behaved plus_S.
-Proof.
-  split. intros a; destruct a; apply reflexivity.
-  split. intros a; destruct a; apply reflexivity.
-  intros. destruct a ; destruct b; destruct a'; destruct b';
-  inversion H0; inversion H; reflexivity.
-Qed.
-
-Require Classifier.
-Module  Cl := Classifier.MakeClassifier (P) (A_as_Action).
-Include Cl.
+Module Import Cl := Classifier.MakeClassifier (HFT_Impl).
 
 Fixpoint eval_S (pkt : pkt) (share : S) := match share with
-  | nil => ActionUnit
+  | nil => NoAction
   | (m, a) :: tl => match is_match pkt m with
     | true => plus_S a (eval_S pkt tl)
     | false => eval_S pkt tl
@@ -126,7 +265,7 @@ Fixpoint eval_S (pkt : pkt) (share : S) := match share with
 Fixpoint eval_T (pkt : pkt) (t : T) := match t with
   | Tree share subtrees => 
       plus_P (eval_S pkt share)
-             (fold_right plus_S ActionUnit (map (eval_T pkt) subtrees))
+             (fold_right plus_S NoAction (map (eval_T pkt) subtrees))
 end.
 
 Fixpoint lin_S (share : S) := match share with
@@ -140,4 +279,161 @@ Fixpoint lin_T (tree : T) := match tree with
             (fold_right (union plus_S) nil (map lin_T subtrees))
 end.
 
-End Make.
+Section Correctness.
+
+ Hint Constructors wf_tree T A.
+
+  Section WellFormedness.
+
+  Fixpoint height (tree : T) : nat := match tree with
+    | Tree _ children => 1 + fold_right max 0 (map height children)
+  end.
+
+  Hint Immediate le_or_lt : arith.
+
+  Lemma max_le : forall (l m n : nat),
+    max l m <= n ->
+    l <= n /\ m <= n.
+  Proof with (auto with arith).
+  intros. 
+  assert (l <= m \/ m < l) as [H0 | H1]...
+  assert (max l m = m)... crush.
+  assert (max l m = l)... crush.
+  Qed.
+
+  Hint Resolve max_le succ_max_distr: arith.
+
+  Lemma split_height: forall (s : S) (a : T) (L : list T) (n : nat),
+    height (Tree s (a :: L)) <= n ->
+    height (Tree s L) <= n.
+  Proof with auto with arith.
+  intros.
+  generalize dependent a.
+  induction L; intros; crush.
+  rewrite -> succ_max_distr in H.
+  apply max_le in H.
+  crush.
+  Qed.
+
+  Lemma height_list : forall (lst : list T) (n : nat) (t : T),
+    fold_right max 0 (map height lst) <= n ->
+    In t lst ->
+    height t <= n.
+  Proof with crush.
+  intros.
+  induction lst...
+  apply max_le in H...
+  apply IHlst in H1...
+  apply max_le in H...
+  Qed.
+
+  Hint Resolve height_list.
+
+  Lemma decreasing_height: forall (s : S) (lst : list T) (t : T) (n : nat),
+    height (Tree s lst) <= n ->
+  In t lst ->
+  height t < n.
+  Proof with eauto with arith.
+  intros.
+  generalize dependent lst.
+  induction n; intros...
+  Qed.
+
+  Hint Resolve decreasing_height.
+
+  Lemma wf_exists_aux : forall (tree : T) (n : nat),
+    height tree <= n -> wf_tree n tree.
+  Proof with simpl; (eauto with arith).
+  intros.
+  generalize dependent tree.
+  induction n; intros; destruct tree.
+  crush.
+  (* Inductive *)
+  apply wf_tree_lst.
+  intros. apply IHn. crush.
+  assert (height t' < Datatypes.S n)...
+  Qed.
+
+  Lemma wf_exists : forall (tree : T),
+    wf_tree (height tree) tree.
+  Proof. auto using wf_exists_aux. Qed.
+
+End WellFormedness.
+
+Hint Resolve inter_elim union_comm.
+
+Open Local Scope equiv_scope.
+
+Lemma flatten_eval_S : forall (share : S) (pkt : pkt),
+  eval_S pkt share === scan pkt (lin_S share).
+Proof with auto.
+  intros share pkt.
+  intros.
+  induction share.
+  (* Base case: empty share *)
+  crush. apply reflexivity.
+  (* Inductive case *)
+  simpl.
+  destruct a.
+  remember (is_match pkt p).
+  destruct b.
+  (* Case: matches at head *)
+  assert (scan pkt (union plus_S ((p,a)::nil) (lin_S share)) ===
+          plus_S (scan pkt ((p,a)::nil)) (scan pkt (lin_S share))).
+    apply union_comm... apply well_behaved_plus_S.
+  rewrite -> H.
+  simpl. 
+  assert (is_match = HFT_Impl.is_match)...
+  rewrite <- H0.
+  rewrite <- Heqb.
+  apply well_behaved_plus_S... apply reflexivity.
+  (* Case: does not match at head *)
+  unfold union. rewrite inter_elim... simpl. 
+  assert (is_match = HFT_Impl.is_match)...
+  rewrite <- H.
+  rewrite <- Heqb...
+Qed.
+
+Notation "x +P y" := (plus_P x y) (at level 50, left associativity).
+Notation "x +C y" := (plus_S x y) (at level 50, left associativity).
+
+Lemma flatten_eval_T : forall (n : nat) (tree : T) (pkt : pkt),
+  wf_tree n tree ->
+  eval_T pkt tree === scan pkt (lin_T tree).
+Proof with simpl; auto.
+  intros n tree pkt H.
+  generalize dependent tree.
+  induction n.
+  intros; inversion H.
+(* Inductive case *)
+intros.
+destruct tree.
+simpl.  
+rewrite -> union_comm...
+assert (eval_S pkt s === scan pkt (lin_S s)).
+  apply flatten_eval_S...
+  apply well_behaved_plus_P...
+  clear H0.
+  induction l... 
+  apply reflexivity.
+  rewrite -> union_comm...
+  assert (eval_T pkt a === scan pkt (lin_T a)).
+    apply IHn. inversion H. crush.
+  assert (fold_right plus_S NoAction (map (eval_T pkt) l) ===
+          scan pkt (fold_right (union plus_S) nil (map lin_T l))).
+    apply IHl. intros. apply wf_tree_lst. inversion H; subst. crush.
+  crush.
+  apply well_behaved_plus_S...
+apply well_behaved_plus_S.
+apply well_behaved_plus_P.
+Qed.
+
+Lemma eval_scan_eq : forall (n : nat) (tree : T) (pkt : pkt),
+  eval_T pkt tree === scan pkt (lin_T tree).
+Proof with auto.
+intros.
+assert (wf_tree (height tree) tree). apply wf_exists.
+apply flatten_eval_T with (n := height tree)...
+Qed.
+
+End Correctness.
