coq/Impl.v
@@ -1,7 +1,28 @@
-Module Type Packet.
+Require Import Coq.Init.Datatypes.
+Require Import Coq.Lists.List.
+Require Import Coq.Arith.MinMax.
+Require Import Coq.Classes.Equivalence.
+Require Import Omega.
+Require Import CpdtTactics.
 
+Set Implicit Arguments.
+Open Local Scope equiv_scope.
+
+Module Type IMPL.
+
+  Parameter A : Type.
   Parameter pkt : Set.
   Parameter pat : Set.
+
+  Parameter ActionUnit: A.
+  Parameter equiv : A -> A -> Prop.
+
+  Declare Instance A_Equivalence : Equivalence equiv.
+
+  Definition well_behaved (f : A -> A -> A) : Prop :=
+    (forall (a : A), f a ActionUnit === a) /\
+    (forall (a : A), f ActionUnit a === a) /\
+    (forall a a' b b', a === a' -> b === b' -> f a b === f a' b').
 
   Axiom pkt_eq_dec : forall (m1 m2 : pkt), { m1 = m2 } + { m1 <> m2 }.
   Axiom pat_eq_dec : forall (m1 m2 : pat), { m1 = m2 } + { m1 <> m2 }.
@@ -29,7 +50,7 @@ Module Type Packet.
     is_match pkt m1 = true  ->
     is_match pkt m2 = false.
 
- Hint Rewrite pkt_eq_dec pat_eq_dec packet_split
-              no_match_subset_l no_match_subset_r : packet.
-End Packet.
+  Hint Rewrite pkt_eq_dec pat_eq_dec packet_split
+    no_match_subset_l no_match_subset_r : packet.
 
+End IMPL.
